src/Lean/Meta/Tactic/BVDecide/Prover/Cegar.lean
@@ -1,0 +1,41 @@
+/-
+Copyright (c) 2026 Lean FRO, LLC. All rights reserved.
+Released under Apache 2.0 license as described in the file LICENSE.
+Authors: Henrik Böving
+-/
+module
+prelude
+public import Lean.Meta.Tactic.BVDecide.Prover.Cegar.Basic
+public import Lean.Meta.Tactic.BVDecide.Prover.Cegar.BitVec
+public import Lean.Meta.Tactic.BVDecide.Prover.Cegar.Function
+public import Lean.Meta.Tactic.BVDecide.Prover.Cegar.Lemmas
+
+/-!
+TODO
+-/
+
+namespace Lean.Meta.Tactic.BVDecide
+
+open Cegar in
+public def cegarBlaster (ctx : TacticContext) : UnsatProver LratCert := CegarM.run ctx do
+  let mut lastCex := #[]
+  modify fun s => { s with didChange := true }
+  while ← CegarM.getDidChange do
+    if (← processNewHyps) matches .solved then return .ok "" -- TODO
+    CegarM.setDidChange false
+    match ← checkBitVec with
+    | .ok cert =>
+      -- TODO: have to return learned lemmas
+      return .ok cert
+    | .error cex =>
+      lastCex := cex
+      let cex ← CegarM.CounterExample.ofArray cex
+      if ← checkUf cex then continue
+
+  return .error {
+    goal := (← read).goal,
+    unusedHypotheses := (← read).unusedHypotheses,
+    equations := lastCex
+  }
+
+end Lean.Meta.Tactic.BVDecide
