src/Lean/Meta/Tactic/BVDecide/Prover/Cegar/Basic.lean
@@ -1,0 +1,124 @@
+/-
+Copyright (c) 2026 Lean FRO, LLC. All rights reserved.
+Released under Apache 2.0 license as described in the file LICENSE.
+Authors: Henrik Böving
+-/
+module
+prelude
+public import Lean.Meta.Tactic.BVDecide.Prover.Basic
+public import Lean.Meta.Tactic.BVDecide.TacticContext
+public import Lean.Cadical.Basic
+
+/-!
+This module provides the basic infrastructure for the CEGAR (Counter Example Guided Abstraction Refinement)
+solver.
+-/
+
+namespace Lean.Meta.Tactic.BVDecide
+
+open Std.Tactic.BVDecide
+
+namespace CegarM
+
+public structure Context where
+  goal : MVarId
+  unusedHypotheses : Std.HashSet Normalize.Hyp
+  atomsAssignment : Std.HashMap Nat (Nat × Expr × Bool)
+  tacticContext : TacticContext
+
+public structure FunState where
+  congrCache : Std.HashMap Sym.ExprPtr Expr := {}
+
+public structure BitVecState where
+  aig : Std.Sat.AIG BVBit := .empty
+  blastCache : BVExpr.Cache aig := .empty
+  cnfCache : Std.Sat.AIG.toCNF.State aig := .empty aig
+
+public structure TheoryState where
+  funState : FunState := {}
+  bitvecState : BitVecState := {}
+  satSolver : Cadical.Solver
+
+def TheoryState.new : BaseIO TheoryState := do
+  return { satSolver := ← Cadical.Solver.new }
+
+public structure State where
+  satExpr : SatAtBVLogical
+  newHypotheses : Std.HashSet Normalize.Hyp := {}
+  hypQueue : Array Normalize.Hyp := #[]
+  didChange : Bool := true
+  theoryState : TheoryState
+
+end CegarM
+
+public abbrev CegarM (α : Type) := ReaderT CegarM.Context StateRefT CegarM.State LemmaM α
+
+namespace CegarM
+
+public def getReflectionResult : CegarM ReflectionResult := do
+  return {
+    satExpr := (← get).satExpr
+    unusedHypotheses := (← read).unusedHypotheses
+  }
+
+@[inline]
+public def getDidChange : CegarM Bool := return (← get).didChange
+
+@[inline]
+public def setDidChange (v : Bool) : CegarM Unit := modify fun s => { s with didChange := v }
+
+@[inline]
+public def getTheoryState : CegarM TheoryState := return (← get).theoryState
+
+@[inline]
+public def modifyTheoryState (f : TheoryState → TheoryState) : CegarM Unit :=
+  modify fun s => { s with theoryState := f s.theoryState }
+
+@[inline]
+public def pushNewHyp (hyp : Normalize.Hyp) : CegarM Unit :=
+  modify fun s => { s with hypQueue := s.hypQueue.push hyp }
+
+@[inline]
+public def drainNewHyps : CegarM (Array Normalize.Hyp) :=
+  modifyGet fun s => (s.hypQueue, { s with hypQueue := #[] })
+
+@[inline]
+public def getTacticContext : CegarM TacticContext := return (← read).tacticContext
+
+@[inline]
+public def hasRefinementProcedures : CegarM Bool := do
+  let cfg := (← getTacticContext).config
+  return cfg.uf
+
+@[inline]
+public def run (ctx : TacticContext) (x : CegarM (Except CounterExample α)) : UnsatProver α :=
+  fun goal reflectionResult atomsAssignment => do
+    let ctx := {
+      goal := goal
+      unusedHypotheses := reflectionResult.unusedHypotheses
+      atomsAssignment := atomsAssignment
+      tacticContext := ctx
+    }
+    let state := {
+      satExpr := reflectionResult.satExpr
+      theoryState := ← TheoryState.new
+    }
+    StateRefT'.run' (ReaderT.run x ctx) state
+
+public def getSatSolver : CegarM Cadical.Solver := return (← get).theoryState.satSolver
+
+public structure CounterExample where
+  exprCex : Std.HashMap Expr BVExpr.PackedBitVec
+  atomCex : Std.HashMap Nat BVExpr.PackedBitVec
+
+public def CounterExample.ofArray (arr : Array (Expr × BVExpr.PackedBitVec)) : ReifyM CounterExample := do
+  let exprCex := Std.HashMap.ofArray arr
+  let mut atomCex := Std.HashMap.emptyWithCapacity arr.size
+  for (expr, val) in arr do
+    let some atom ← ReifyM.getAtomNumber expr | unreachable!
+    atomCex := atomCex.insert atom val
+  return { exprCex, atomCex }
+
+end CegarM
+
+end Lean.Meta.Tactic.BVDecide
