src/Lean/Meta/Tactic/BVDecide/Prover/Cegar/BitVec.lean
@@ -1,0 +1,100 @@
+/-
+Copyright (c) 2026 Lean FRO, LLC. All rights reserved.
+Released under Apache 2.0 license as described in the file LICENSE.
+Authors: Henrik Böving
+-/
+module
+prelude
+public import Lean.Meta.Tactic.BVDecide.Prover.Cegar.Basic
+import Lean.Meta.Sym.InferType
+import Lean.Meta.Tactic.BVDecide.Prover.Bitblast
+
+/-!
+TODO
+-/
+
+namespace Lean.Meta.Tactic.BVDecide
+
+open Std.Sat
+open Std.Tactic.BVDecide
+open Std.Tactic.BVDecide.Reflect
+
+@[inline]
+def takeBVState : CegarM CegarM.BitVecState := do
+  let state := (← CegarM.getTheoryState).bitvecState
+  CegarM.modifyTheoryState fun ts => { ts with bitvecState := {} }
+  return state
+
+@[inline]
+def setBVState (s : CegarM.BitVecState) : CegarM Unit :=
+  CegarM.modifyTheoryState fun ts => { ts with bitvecState := s }
+
+def pushNewCnf (prevCnfSize : Nat) (current : CNF Nat) : CegarM Unit := do
+  let satSolver ← CegarM.getSatSolver
+  for clause in current.clauses[prevCnfSize...*] do
+    satSolver.clause clause
+
+def getAssignment (aigSize : Nat) : CegarM (Array (Bool × Nat)) := do
+  let satSolver ← CegarM.getSatSolver
+  let mut model := Array.emptyWithCapacity aigSize
+  for idx in 0...aigSize do
+    let value ← satSolver.val idx
+    model := model.push (value, idx)
+  return model
+
+public def Cegar.checkBitVec :
+    CegarM (Except (Array (Expr × BVExpr.PackedBitVec)) LratCert) := do
+  let ctx ← CegarM.getTacticContext
+  let bvExpr := (← get).satExpr.bvExpr
+  let ⟨aig, bbCache, cnfCache⟩ ← takeBVState
+  let prevAigSize := aig.decls.size
+  let blastResult : { ret : Return aig // AIG.IsPrefix aig.decls ret.result.1.aig.decls } ←
+    withTraceNode `Meta.Tactic.bv (fun _ => return "Bitblasting BVLogicalExpr to AIG") do
+      -- lazyPure to prevent compiler lifting
+      IO.lazyPure (fun _ =>
+        let res := bvExpr.bitblastWithCache aig bbCache
+        ⟨res, BVLogicalExpr.bitblastWithCache_isPrefix_aig⟩
+      )
+  let ret := blastResult.1
+  let bbCache := ret.cache
+  let entry := ret.result.1
+  let aig := entry.aig
+  let aigSize := aig.decls.size
+  trace[Meta.Tactic.bv] s!"AIG has {aigSize} nodes, added {aigSize - prevAigSize} nodes this round"
+
+  if ctx.config.graphviz then
+    IO.FS.writeFile ("." / "aig.gv") <| AIG.toGraphviz entry
+
+
+  let prevCnfSize := cnfCache.cnf.clauses.size
+  let cnfCache := cnfCache.cast blastResult.2
+  let cnfCache ←
+    withTraceNode `Meta.Tactic.sat (fun _ => return "Converting AIG to CNF") do
+      -- lazyPure to prevent compiler lifting
+      IO.lazyPure (fun _ => AIG.toCNF' entry cnfCache)
+  let cnfSize := cnfCache.cnf.clauses.size
+  trace[Meta.Tactic.bv] s!"CNF has {cnfSize} clauses, added {cnfSize - prevCnfSize} clauses this round"
+
+  setBVState ⟨entry.aig, bbCache, cnfCache⟩
+
+  pushNewCnf prevCnfSize cnfCache.cnf
+  let satSolver ← CegarM.getSatSolver
+  satSolver.assume entry.ref.gate !entry.ref.invert
+  -- TODO: this needs to be made interruptible
+  let status ← satSolver.solve
+
+  match status with
+  | .satisfiable =>
+    trace[Meta.Tactic.sat] "SAT solver found a counter example."
+    let assignment ← getAssignment aigSize
+    let equations := reconstructCounterExample entry.aig assignment (← read).atomsAssignment
+    return .error equations
+  | .unsatisfiable =>
+    let res ← lratBitblaster ctx (← read).goal (← CegarM.getReflectionResult) (← read).atomsAssignment
+    match res with
+    | .ok cert => return .ok cert
+    | .error _ => throwError m!"Error during proof recovery"
+    throwError m!"SAT solver reports UNSAT"
+  | .unknown => throwError m!"SAT solver timed out"
+
+end Lean.Meta.Tactic.BVDecide
