src/Lean/Meta/Tactic/BVDecide/Prover/Cegar/Function.lean
@@ -1,0 +1,151 @@
+/-
+Copyright (c) 2026 Lean FRO, LLC. All rights reserved.
+Released under Apache 2.0 license as described in the file LICENSE.
+Authors: Henrik Böving
+-/
+module
+prelude
+public import Lean.Meta.Tactic.BVDecide.Prover.Cegar.Basic
+import Lean.Meta.Sym.InferType
+
+/-!
+TODO
+-/
+
+namespace Lean.Meta.Tactic.BVDecide
+
+open Std.Tactic.BVDecide
+
+namespace Cegar
+
+deriving instance Inhabited, BEq, Hashable for Sum
+
+structure FunModel.Entry where
+  -- TODO: bzla caches hashes of `Array BVExpr.PackedBitVec` here
+  map : Std.HashMap (Array (BVExpr.PackedBitVec ⊕ Expr)) (BVExpr.PackedBitVec × Expr)
+  deriving Inhabited
+
+structure FunModel where
+  model : Std.HashMap Sym.ExprPtr FunModel.Entry := {}
+  deriving Inhabited
+
+namespace FunModel
+
+namespace Entry
+
+def new (args : Array (BVExpr.PackedBitVec ⊕ Expr)) (value : BVExpr.PackedBitVec) (atom : Expr) : Entry :=
+  {
+    map := {(args, (value, atom))}
+  }
+
+def insert (entry : Entry) (args : Array (BVExpr.PackedBitVec ⊕ Expr)) (value : BVExpr.PackedBitVec)
+    (atom : Expr) : Entry :=
+  { entry with
+      map := entry.map.insert args (value, atom)
+  }
+
+end Entry
+
+def findConflictWith? (funModel : FunModel) (fn : Expr) (args : Array (BVExpr.PackedBitVec ⊕ Expr))
+    (value : BVExpr.PackedBitVec) : Option Expr := do
+  let key : Sym.ExprPtr := { expr := fn }
+  let entry ← funModel.model[key]?
+  let (value', atom') ← entry.map[args]?
+  if value ≠ value' then
+    return atom'
+  else
+    none
+
+def insert (funModel : FunModel) (fn : Expr) (args : Array (BVExpr.PackedBitVec ⊕ Expr))
+    (value : BVExpr.PackedBitVec) (atom : Expr) : FunModel :=
+  { funModel with
+      model := funModel.model.alter ⟨fn⟩
+        fun
+          | some entry => some <| entry.insert args value atom
+          | none => some <| Entry.new args value atom
+  }
+
+end FunModel
+
+def addFunctionCongruenceLemma (lhs rhs : Expr) (mask : Array Bool) (pattern : Expr) :
+    CegarM Unit := do
+  let lhsArgs := lhs.getAppArgs
+  let rhsArgs := rhs.getAppArgs
+  let mut congrLemma ← getCongrLemmaForPattern pattern
+  for lhsArg in lhsArgs, rhsArg in rhsArgs, m in mask do
+    unless m do continue
+    congrLemma := mkApp2 congrLemma lhsArg rhsArg
+  congrLemma ← Sym.share congrLemma
+  let congrStatement ← Sym.inferType congrLemma
+  trace[Meta.Tactic.bv] m!"{congrStatement}"
+  CegarM.pushNewHyp {
+    name := `congr
+    type := congrStatement
+    value := congrLemma
+    source := .cegar
+  }
+  CegarM.setDidChange true
+where
+  getCongrLemmaForPattern (pattern : Expr) : CegarM Expr := do
+    let key : Sym.ExprPtr := { expr := pattern }
+    if let some lem := (← CegarM.getTheoryState).funState.congrCache[key]? then
+      return lem
+    else
+      let lem ← mkCongrLemmaForPattern pattern
+      CegarM.modifyTheoryState fun ts =>
+        { ts with funState.congrCache := ts.funState.congrCache.insert key lem}
+      return lem
+
+  mkCongrLemmaForPattern (pattern : Expr) : CegarM Expr := do
+    lambdaTelescope pattern fun lhsArgs _ => do
+    lambdaTelescope pattern fun rhsArgs _ => do
+      let mut equalityDecls := #[]
+      for lhsArg in lhsArgs, rhsArg in rhsArgs do
+        equalityDecls := equalityDecls.push (.anonymous, ← mkEq lhsArg rhsArg)
+      withLocalDeclsDND equalityDecls fun equalities => do
+        let mut lem ← mkAppM ``congrArg #[pattern, equalities[0]!]
+        for equality in equalities[1...*] do
+          lem ← mkAppM ``congr #[lem, equality]
+        let mut fvars := #[]
+        for lhsArg in lhsArgs, rhsArg in rhsArgs do
+          fvars := fvars.push lhsArg |>.push rhsArg
+        fvars := fvars ++ equalities
+        mkLambdaFVars fvars lem
+
+open Std.Tactic.BVDecide.EfficientEval in
+public def checkUf (cex : CegarM.CounterExample) : CegarM Bool :=
+  withTraceNode `Meta.Tactic.bv (fun _ => return m!"UF conflict detection") do
+  unless (← CegarM.getTacticContext).config.uf do return false
+  let funState := (← getThe BVDecide.State).theoryState.funState
+  let mut funModel : FunModel := {}
+  for funAtom in funState.atoms, mask in funState.masks, funPattern in funState.patterns do
+    let args ← evalArgs funAtom.getAppArgs mask
+    let value := cex.exprCex[funAtom]!
+    trace[Meta.Tactic.bv] m!"Checking: {funAtom}, value: {value.bv}, pattern: {funPattern}"
+    if let some conflict := funModel.findConflictWith? funPattern args value then
+      assert! funAtom != conflict
+      trace[Meta.Tactic.bv] m!"Detected UF conflict on: {funAtom} vs {conflict}"
+      addFunctionCongruenceLemma funAtom conflict mask funPattern
+    else
+      funModel := funModel.insert funPattern args value funAtom
+  return ← CegarM.getDidChange
+where
+  evalArgs (args : Array Expr) (mask : Array Bool) : CegarM (Array (BVExpr.PackedBitVec ⊕ Expr)) := do
+    args.mapIdxM fun idx arg => do
+      if mask[idx]! then
+        if (← isValidBitVecAtom arg).isSome then
+          let some reified ← ReifiedBVExpr.of arg | unreachable!
+          let res := BVExpr.evalEfficient (cex.atomCex.getD · ⟨0#1⟩) reified.bvExpr
+          return .inl ⟨res⟩
+        else if ← isValidBoolAtom arg then
+          let some reified ← ReifiedBVLogical.of arg | unreachable!
+          let res := BVLogicalExpr.evalEfficient (cex.atomCex.getD · ⟨0#1⟩) reified.bvExpr
+          return .inl ⟨BitVec.ofBool res⟩
+        else
+          unreachable!
+      else
+        return .inr arg
+
+end Cegar
+
+end Lean.Meta.Tactic.BVDecide
