src/Lean/Meta/Tactic/BVDecide/Prover/Cegar/Lemmas.lean
@@ -1,0 +1,49 @@
+/-
+Copyright (c) 2026 Lean FRO, LLC. All rights reserved.
+Released under Apache 2.0 license as described in the file LICENSE.
+Authors: Henrik Böving
+-/
+module
+prelude
+public import Lean.Meta.Tactic.BVDecide.Prover.Cegar.Basic
+import Lean.Meta.Tactic.BVDecide.Normalize
+import Lean.Meta.Tactic.Grind.Main
+
+/-!
+TODO
+-/
+
+namespace Lean.Meta.Tactic.BVDecide
+
+public inductive ProcessHypResult where
+  | solved
+  | newHyps
+  | none
+
+public def Cegar.processNewHyps : CegarM ProcessHypResult := do
+  let hypQueue ← CegarM.drainNewHyps
+  if hypQueue.isEmpty then return .none
+  let params ← Grind.mkDefaultParams {}
+  -- TODO: think about carrying over caches
+  let target := .mvarIdTarget (← read).goal
+  let ctx := (← CegarM.getTacticContext).preProcessContext
+  let (solved, state) ← Grind.GrindM.run (params := params) <| Normalize.PreProcessM.run ctx target do
+    Normalize.bvNormalize hypQueue
+  if solved then return .solved
+  let hypQueue := state.hypotheses
+
+  let mut sats := #[]
+  for hyp in hypQueue do
+    checkSystem "bv_decide"
+    -- TODO: think about repeated lemmas
+    if let (some reflected, lemmas) ← (SatAtBVLogical.of hyp).run then
+      sats := (sats ++ lemmas).push reflected
+    else
+      throwError m!"Failed to reify CEGAR lemma {hyp}"
+
+  let sat ← sats.foldlM (init := (← get).satExpr) (SatAtBVLogical.and · ·)
+  modify fun s => { s with satExpr := sat, newHypotheses := s.newHypotheses.insertMany hypQueue }
+  return .newHyps
+
+end Lean.Meta.Tactic.BVDecide
+
