src/Lean/Meta/Tactic/BVDecide/Reflect/SatAtBVLogical.lean
@@ -59,7 +59,7 @@ public def and (x y : SatAtBVLogical) : ReifyM SatAtBVLogical := do
       (mkConst ``BVLogicalExpr.sat_and)
       x.expr
       y.expr
-      (← M.atomsAssignment)
+      (← ReifyM.atomsAssignment)
       (← x.satAtAtoms)
       (← y.satAtAtoms)
   return ⟨bvExpr, proof, expr⟩
@@ -69,7 +69,7 @@ public def proveFalse (x : SatAtBVLogical) (h : Expr) : ReifyM Expr := do
   if (← get).atoms.isEmpty then
     throwError "Unable to identify any relevant atoms."
   else
-    let atomsList ← M.atomsAssignment
+    let atomsList ← ReifyM.atomsAssignment
     let evalExpr ← Sym.share <| mkApp2 (mkConst ``BVLogicalExpr.eval) atomsList x.expr
     return mkApp3
       (mkConst ``Std.Tactic.BVDecide.Reflect.Bool.false_of_eq_true_of_eq_false)
