src/Std/Tactic/BVDecide/Bitblast/EfficientEval.lean
@@ -1,0 +1,90 @@
+/-
+Copyright (c) 2026 Lean FRO, LLC. All rights reserved.
+Released under Apache 2.0 license as described in the file LICENSE.
+Authors: Henrik Böving
+-/
+module
+prelude
+public import Std.Tactic.BVDecide.Bitblast.BVExpr.Basic
+import Init.System.IO
+import Std.Tactic.BVDecide.Bitblast.BVExpr.Circuit.Impl.Expr
+import Std.Data.HashMap.Basic
+
+
+/-!
+This module contains efficient evaluation for the reification data types of `bv_decide`, used for
+evaluating counterexamples during CEGAR.
+-/
+
+namespace Std.Tactic.BVDecide
+
+namespace EfficientEval
+
+structure Cache where
+  exprMap : Std.DHashMap BVExpr.Cache.Key (fun k => BitVec k.w) := {}
+
+abbrev EvalM (σ : Type) := ReaderT (Nat → BVExpr.PackedBitVec) StateRefT Cache (ST σ)
+
+@[inline]
+def EvalM.run (assign : Nat → BVExpr.PackedBitVec) (x : (σ : Type) → EvalM σ α) : α :=
+  runST fun σ =>
+    let x : EvalM σ α := x σ
+    StateRefT'.run' (ReaderT.run x assign) {}
+
+partial def BVExpr.evalEfficientM (expr : BVExpr w) : EvalM σ (BitVec w) := do
+  let key := ⟨w, expr⟩
+  if let some res := (← get).exprMap.get? key then
+    return res
+  else
+    let res ← go expr
+    modify fun s => { s with exprMap := s.exprMap.insert key res }
+    return res
+where
+  go {w : Nat} : BVExpr w → EvalM σ (BitVec w)
+    | .var idx => do
+      let packedBv := (← read) idx
+      /-
+      This formulation improves performance, as in a well formed expression the condition always holds
+      so there is no need for the more involved `BitVec.truncate` logic.
+      -/
+      if h : packedBv.w = w then
+        return h ▸ packedBv.bv
+      else
+        return packedBv.bv.truncate w
+    | .const val => return val
+    | .extract start len expr => return BitVec.extractLsb' start len (← evalEfficientM expr)
+    | .bin lhs op rhs => return op.eval (← evalEfficientM lhs) (← evalEfficientM rhs)
+    | .un op operand => return op.eval (← evalEfficientM operand)
+    | .append lhs rhs h => return h ▸ ((← evalEfficientM lhs) ++ (← evalEfficientM rhs))
+    | .replicate n expr h => return h ▸ (BitVec.replicate n (← evalEfficientM expr))
+    | .shiftLeft lhs rhs => return (← evalEfficientM lhs) <<< (← evalEfficientM rhs)
+    | .shiftRight lhs rhs => return (← evalEfficientM lhs) >>> (← evalEfficientM rhs)
+    | .arithShiftRight lhs rhs => return BitVec.sshiftRight' (← evalEfficientM lhs) (← evalEfficientM rhs)
+
+partial def BVPred.evalEfficientM (expr : BVPred) : EvalM σ Bool := do
+  match expr with
+  | .bin lhs op rhs => return op.eval (← BVExpr.evalEfficientM lhs) (← BVExpr.evalEfficientM rhs)
+  | .getLsbD expr idx => return (← BVExpr.evalEfficientM expr).getLsbD idx
+
+partial def BVLogicalExpr.evalEfficientM (expr : BVLogicalExpr) : EvalM σ Bool := do
+  match expr with
+  | .literal l => BVPred.evalEfficientM l
+  | .const b => return b
+  | .not x => return !(← evalEfficientM x)
+  | .gate g x y => return g.eval (← evalEfficientM x) (← evalEfficientM y)
+  | .ite d l r => bif (← evalEfficientM d) then evalEfficientM l else evalEfficientM r
+
+public def BVExpr.evalEfficient (assign : Nat → BVExpr.PackedBitVec) (expr : BVExpr w) :
+    BitVec w :=
+  EvalM.run assign (fun σ => BVExpr.evalEfficientM (σ := σ) expr)
+
+public def BVPred.evalEfficient (assign : Nat → BVExpr.PackedBitVec) (expr : BVPred) : Bool :=
+  EvalM.run assign (fun σ => BVPred.evalEfficientM (σ := σ) expr)
+
+public def BVLogicalExpr.evalEfficient (assign : Nat → BVExpr.PackedBitVec)
+    (expr : BVLogicalExpr) : Bool :=
+  EvalM.run assign (fun σ => BVLogicalExpr.evalEfficientM (σ := σ) expr)
+
+end EfficientEval
+
+end Std.Tactic.BVDecide
