tests/elab/bv_uf.lean
@@ -1,13 +1,27 @@
 import Std.Tactic.BVDecide
 
+set_option trace.Meta.Tactic.bv true in
+example (f : BitVec 8 → BitVec 8) (x y : BitVec 8) (h : x = y) :
+    f x = f y := by
+  bv_decide +uf
+
+example (x y : BitVec 8) (h : x ^^^ y = x) :
+    x = 0 ∨ y = 0 := by
+  bv_decide +uf
 
 set_option trace.Meta.Tactic.bv true in
 example (f g : BitVec 8 → BitVec 8) (x y : BitVec 8) (h : x = y) :
     f (g x) = f (g y) := by
-  bv_decide
+  bv_decide +uf
 
+set_option trace.Meta.Tactic.bv true in
+example (f g : {w : Nat} → BitVec w → BitVec w) (x y : BitVec 8) (h : x = y) :
+    f (g x) = f (g y) := by
+  bv_decide +uf
+
+/-
 set_option trace.Meta.Tactic.bv true in
 example (f g : BitVec 8 → BitVec 8) (x y : BitVec 8) (h : x = y) :
     f (g (if x = 0 then 0 else f x)) = f (g y) := by
-  bv_decide
-
+  bv_decide +uf
+-/
